\documentclass{article}
\usepackage{amsmath}
\usepackage{amsfonts}
\usepackage{amssymb}

\begin{document}

\title{Solution to the Differential Equation $y'' + y' + y + t = 0$}
\author{}
\date{}
\maketitle

\section*{Problem}
Solve the differential equation:
\begin{equation}
y'' + y' + y + t = 0
\end{equation}

\section*{Solution}
First, we solve the homogeneous part of the differential equation:
\begin{equation}
y'' + y' + y = 0
\end{equation}

The characteristic equation is:
\begin{equation}
r^2 + r + 1 = 0
\end{equation}
Solving this characteristic equation, we get the roots:
\begin{equation}
r = \frac{-1 \pm \sqrt{-3}}{2} = \frac{-1 \pm \sqrt{3}i}{2}
\end{equation}

Thus, the general solution to the homogeneous equation is:
\begin{equation}
y_h(t) = e^{-\frac{t}{2}} \left( C_1 \sin\left(\frac{\sqrt{3}t}{2}\right) + C_2 \cos\left(\frac{\sqrt{3}t}{2}\right) \right)
\end{equation}

Now, we find a particular solution to the non-homogeneous equation. We try a particular solution of the form:
\begin{equation}
y_p(t) = At + B
\end{equation}

Substituting $y_p(t)$ into the non-homogeneous differential equation:
\begin{align}
y_p'' + y_p' + y_p + t &= 0 \\
0 + A + (At + B) + t &= 0 \\
(1+A)t + (A + B) &= 0
\end{align}

Equating coefficients, we get:
\begin{align}
1 + A &= 0 \\
A + B &= 0
\end{align}

Solving these equations, we find:
\begin{align}
A &= -1 \\
B &= 1
\end{align}

Thus, the particular solution is:
\begin{equation}
y_p(t) = -t + 1
\end{equation}

Combining the homogeneous and particular solutions, we get the general solution:
\begin{equation}
y(t) = y_h(t) + y_p(t) = e^{-\frac{t}{2}} \left( C_1 \sin\left(\frac{\sqrt{3}t}{2}\right) + C_2 \cos\left(\frac{\sqrt{3}t}{2}\right) \right) - t + 1
\end{equation}

Therefore, the solution to the differential equation is:
\begin{equation}
y(t) = -t + \left( C_1 \sin\left(\frac{\sqrt{3}t}{2}\right) + C_2 \cos\left(\frac{\sqrt{3}t}{2}\right) \right) e^{-\frac{t}{2}} + 1
\end{equation}

\end{document}
